Veritas.Verifier.Blum.fsti
@@ -147,6 +147,12 @@ val lemma_evict_before_add2 (#p:pos) (itsl: its_log p) (i:seq_index itsl{is_blum
          (ensures (MS.mem (blum_add_elem (index itsl i)) (ts_evict_set itsl) =
                    MS.mem (blum_add_elem (index itsl i)) (ts_evict_set (its_prefix itsl i))))
 
+val lemma_evict_before_add3 (#p:pos) (itsl: its_log p) (i: seq_index itsl) (j:seq_index itsl):
+  Lemma (requires (is_blum_add (index itsl i) /\
+                   is_blum_evict (index itsl j) /\
+                   blum_add_elem (index itsl i) = blum_evict_elem itsl j))
+        (ensures (j < i))
+
 (* for an eac ts log, if the eac state of a key k is instore, the count of blum evicts 
  * is the same of blum adds for that key *)
 val lemma_evict_add_count_same (#p:pos) (itsl: eac_ts_log p) (k:key):
@@ -189,3 +195,11 @@ val lemma_eac_evicted_blum_implies_previous_evict (#p:pos) (itsl: its_log p) (k:
                   is_blum_evict (index itsl (last_idx_of_key itsl k)) /\
                   blum_evict_elem itsl (last_idx_of_key itsl k) = 
                   to_blum_elem (eac_state_of_key itsl k) k))
+
+(* if we provide two indexes having the same add element then the membership of the element in the 
+ * add set is at least two *)
+val lemma_add_set_mem (#p:pos) (itsl: its_log p) (i: seq_index itsl) (j:seq_index itsl{j <> i}):
+  Lemma (requires (is_blum_add (index itsl i) /\
+                   is_blum_add (index itsl j) /\
+                   blum_add_elem (index itsl i) = blum_add_elem (index itsl j)))
+        (ensures (MS.mem (blum_add_elem (index itsl i)) (ts_add_set itsl) >= 2))
